Compile parent traits of traits, and omit duplicates. Compile inherited trait members only in classes. Use appropriate type substitutions when verifying definite assignments. Move some tests from TraitOverride2.dfy to TraitVerify.dfy.

Source/Dafny/Compiler.cs
@@ -707,7 +707,7 @@ namespace Microsoft.Dafny {
           } else if (d is TraitDecl) {
             // writing the trait
             var trait = (TraitDecl)d;
-            var w = CreateTrait(trait.CompileName, trait.IsExtern(out _, out _), trait.TypeArgs, null, null, wr);
+            var w = CreateTrait(trait.CompileName, trait.IsExtern(out _, out _), trait.TypeArgs, trait.ParentTypeInformation.UniqueParentTraits(), trait.tok, wr);
             CompileClassMembers(trait, w);
           } else if (d is ClassDecl) {
             var cl = (ClassDecl)d;
@@ -725,7 +725,7 @@ namespace Microsoft.Dafny {
               }
             }
             if (include) {
-              var cw = CreateClass(IdName(cl), classIsExtern, cl.FullName, cl.TypeArgs, cl.ParentTraits, cl.tok, wr);
+              var cw = CreateClass(IdName(cl), classIsExtern, cl.FullName, cl.TypeArgs, cl.ParentTypeInformation.UniqueParentTraits(), cl.tok, wr);
               CompileClassMembers(cl, cw);
               cw.Finish();
             } else {
@@ -946,7 +946,7 @@ namespace Microsoft.Dafny {
 
       List<MemberDecl> inheritedMembers;
       Dictionary<TypeParameter, Type> typeMap;
-      if (c is TopLevelDeclWithMembers cl) {
+      if (c is TopLevelDeclWithMembers cl && !(c is TraitDecl)) {
         inheritedMembers = cl.InheritedMembers;
         typeMap = cl.ParentFormalTypeParametersToActuals;
       } else {
@@ -1044,7 +1044,9 @@ namespace Microsoft.Dafny {
       }
 
       foreach (MemberDecl member in c.Members) {
-        if (member is Field) {
+        if (c is TraitDecl && member.OverriddenMember != null) {
+          // emit nothing in the trait; this member will be emitted in the classes that extend this trait
+        } else if (member is Field) {
           var f = (Field)member;
           if (f.IsGhost) {
             // emit nothing, but check for assumes
