Test/traits/TraitVerify.dfy
@@ -34,3 +34,87 @@ method R(a: A) {
   var t: A?;
   t := a;
 }
+
+// -----------------------------------------------------
+
+module TestParentTraitRelation {
+  trait BTrait {
+    ghost var Repr: set<object>
+    predicate Valid()
+      reads this, Repr
+      ensures Valid() ==> this in Repr
+    method SomeMethod()
+      requires Valid()
+      modifies Repr
+      ensures Valid() && fresh(Repr - old(Repr))
+  }
+
+  trait CTrait {
+    ghost var Repr: set<object>
+    predicate Valid()
+      reads this, Repr
+      ensures Valid() ==> this in Repr
+  }
+
+  method doSomething(b: BTrait, c: BTrait)
+    requires b.Valid() && c.Valid() && b.Repr !! c.Repr
+    modifies b.Repr
+    ensures b.Valid() && c.Valid()
+  {
+    b.SomeMethod();
+  }
+}
+
+// -----------------------------------------------------
+
+module TraitsExtendingTraits {
+  trait A<Y0, Y1> {
+    var y0: Y0
+    const y1: Y1
+  }
+
+  trait K<Y> extends A<Y, int> {
+    const k := y1
+  }
+
+  class G<X> extends K<X> {
+    constructor () {
+    }  // error: must assign to y0 (but assigning to y1 is not necessary)
+  }
+
+  // ----
+
+  trait B {
+    method Get() returns (x: int)
+  }
+  trait M extends B {
+    method Get() returns (x: int)
+      ensures 0 <= x <= 20
+    {
+      return 15;
+    }
+  }
+  trait N extends B {
+  }
+  class H extends M, N {
+    constructor () { }
+  }
+  method BMNH() {
+    var h := new H();
+    var b: B, m: M, n: N := h, h, h;
+
+    if
+    case true =>
+      var x := h.Get();
+      assert x <= 20;
+    case true =>
+      var x := b.Get();
+      assert x <= 20;  // error: this is not provable
+    case true =>
+      var x := m.Get();
+      assert x <= 20;
+    case true =>
+      var x := n.Get();
+      assert x <= 20;  // error: this is not provable
+  }
+}
